last state

meta-prog/lecture.lean
@@ -17,74 +17,319 @@ variables and meta variables.
 #print name
 #print level
 
+namespace lecture
+
+open expr tactic
+
+
+
+
+
+
+
+
+
+
+
+
+section expr -- let's construct some terms
+
+-- A very simple definition: Prop, i.e. Sort 0
+meta def prop : expr := sort level.zero
+
+run_cmd trace prop
+-- outputs: Prop ← this is the object logic Prop
+
+
+
+
+
+
+
+
+
+
+
+
+
+-- Let's represent logic as meta expressions:
+
+meta def or_ (a b : expr) : expr :=
+((const `or []).app a).app b
+
+meta def and_ (a b : expr) : expr :=
+((const `and []).app a).app b
+
+meta def true_ : expr :=
+const `true []
+
+meta def false_ : expr :=
+const `false []
+
+meta def imp_ (a b : expr) : expr :=
+pi `hyp binder_info.default a b
+
+
+
+
+
+
+
+
+
+
+
+
+
+run_cmd trace (imp_ false_ true_)
+
+run_cmd trace (and_ true_ (and_ false_ false_))
+
+
+
+
+
+
+
+
+
+
+
+
+
+-- Use antiquotations `(e) as easier way to write expressions:
+
+run_cmd trace `(true ∧ false)
+
+meta def and_aq (a b : expr) : expr :=
+`(%%a ∧ %%b)
+
+
+
+
+
+
+
+
+
+
+
+
+
+-- Problem: When we use %%a the type must be known by context
+--   this will relaxed in tactic mode...
+meta def imp_aq (a b : expr) : expr :=
+`((%%a : Prop) → (%%b : Prop))
+
+meta def nat_add_aq (a b : expr) : expr :=
+`(%%a + %%b : ℕ)
+
+
+
+
+
+
+
+
+
+
+
+
+
+
+/- Example: project the i-th or in a sequence of
+  p₀ ∨ (p₁ ∨ (⋯ ∨ pn))
+
+We can use antiquotation for pattern matching
+-/
+meta def project_or : expr → ℕ → expr
+| `(%%a ∧ %%b) 0       := a
+| `(%%a ∧ %%b) (n + 1) := project_or b n
+| e            _       := e
+
+
+
+
+#check @and.left
+/- Example: proof the i-th disjunct given a sequence
+  p₀ ∧ (p₁ ∧ (⋯ ∧ p_n)) → p_i
+-/
+meta def and_in : expr → ℕ → expr → expr
+| `(%%a ∧ %%b) 0       h := `(@and.left %%a %%b %%h)
+| `(%%a ∧ %%b) (n + 1) h := and_in b n `(@and.right %%a %%b %%h)
+| e            _       h := h
+
+
+
+
+
+
+example {p q r : Prop} (h : p ∧ (q ∧ r)) : q :=
+by do
+  h ← get_local `h,
+  t ← infer_type h,
+  trace t,
+  trace (and_in t 1 h),
+  infer_type (and_in t 1 h) >>= trace,
+  tactic.exact (and_in t 1 h)
+
+end expr
+
+
+
+
+
+
+/- Variables / Constant -/
+section vars
+
+/- declared constant:
+Constant refering to global declarations, and can be looked up in the name space. They are also
+universe parametric, so a list of concrete universe levels needs to be provided. -/
+#check (const : name → list level → expr)
+
+/- bound variable:
+de-Bruijn indexed, i.e. just a natural number giving the distance to the corresponding lambda / pi.
+-/
+#check (var : ℕ → expr)
+
+/- local constant:
+Are arbitrarily created, but we need a unique name.
+-/
+#check (local_const : name → name → binder_info → expr → expr)
+
+/- meta variable:
+Represent holes in our proof / term. Represent the goals we want to solve, or holes to fill in when
+unifying two terms.
+-/
+#check (mvar : name → name → expr → expr)
+
 /-
+Using bound variables with de-Bruijn indices and free variables with names is called a
+**locally nameless representation**.
 
-The `tactic` monad allows us to construct expressions, and interact with the user. It also gives us
-access to Lean's global data, i.e. all declarations (axioms, constant & inductive definitions,
-names), attribute lists, options, etc...
+Local variables and Meta variables exist also for universe levels. They are only used to
+construct a term. In the final declaration local and meta variables do not occur anymore.
 
+Local variables are often used to **walk** into a binder (i.e. a Π or a λ): a new unique name is
+used to create a `local_const` expression using the pretty print name, the binder information, and
+the type of the bound variable. In the expression itself the bound variable is replaced by the local
+variable.
+
+In the interface `expr` is often used instead of the name of the local constant, as `expr` contains
+all necessary information.
 -/
 
-#check tactic
-#print prefix tactic
-#check declaration
-#print prefix declaration
+section deBruijn
+-- Let's play with binders:
 
-/-
+meta def id (α : expr) : expr :=
+lam `a binder_info.default α (var 0)
 
-`expr (elaborated : bool) : Type`
+meta def flip (α : expr) (f : expr) : expr :=
+lam `a binder_info.default α (lam `b binder_info.default α ((f.app (var 0)).app (var 1)))
 
-`elaborated`: is true if the term is fully elaborated, i.e. constants are fully applied, and
-  resolved.
+run_cmd trace (id (const `nat []))
 
-`expr ff` are also called pre-elaborated or `pexpr`. They contain a lot of macros from the parser
-for things which need to be decided, found etc. by the elaborator. The idea is to carry this data
-around until we are in a context where they can be elaborated.
+run_cmd trace (flip (const `nat []) `((+) : ℕ → ℕ → ℕ))
 
-Example:
+meta def forall_prop (e : expr) : expr :=
+pi `a binder_info.default (sort level.zero) e
+
+run_cmd trace (forall_prop (var 0))
+run_cmd trace (forall_prop (imp_ (var 0) true_))
+run_cmd trace (forall_prop (imp_ false_ (var 0))) -- oops
+run_cmd trace (forall_prop (imp_ false_ (var 1)))
+
+meta def imp' (a b : expr) : expr :=
+pi `hyp binder_info.default a (b.lift_vars 0 1)
+
+run_cmd trace (forall_prop (imp' false_ (var 0)))
+
+-- Lean does it right
+run_cmd trace (forall_prop (imp_aq false_ (var 0)))
+
+end deBruijn
+
+
+
+
+
+
+
+section locally_nameless
+
+/- local variables ⇔ bound variables
+
+expr.abstract_local C[local_const n _ _ _] n ~> C[var 0]
+expr.instantiate_var C[var 0] t ~> C[t]
 -/
+#check expr.abstract_local
+#check expr.instantiate_var
 
-example : ∀a:ℕ, a ≤ a ∧ a ≤ a :=
-begin
-  intro a,
-  split; exact le_refl _
-end
 
-/-
 
-The interesting part is: at which time is `le_refl _` elaborated, i.e. when does Lean try to figure
-out what its implicit parameters, its type class instances, and what to fill in at `_`. If it would
-try it already at the parsing time it would fail, `exact` doesn't gice us any information at all.
 
-Even more interesting: `exact` gets executed twice! There is no unique elaborated term which would fit!
 
-The solution: Lean passes pre-elaborated terms to tactics!
- E.g. the `exact` tactic gets `le_refl _` as a pre-elaborated term.
- Then `exact` produces the term: `le_refl _ : a ≤ a` and lets it elaborate.
- In our example this happens two times.
 
-Unfortunately, pre-elaborated terms usually contain a lot of macros and other things which we
-can not access through Lean's `expr`/`tactic` interface. What we can do is: bring the term in the
-right context and tell the elaborator **how** to elaborate it (generating meta-variables / subgoals).
 
+/- instantiate a local constant with a term
+
+expr.instantiate_local n t C[local_const n _ _ _] ~> C[t]
 -/
+#check expr.instantiate_local
+#check expr.instantiate_locals
 
-example : true := by do
-  e ← return ``(0 + @has_one.one ℤ int.has_one),
-  tactic.trace "e",
-  tactic.trace e.to_raw_fmt,
-  e' ← tactic.to_expr e,
-  tactic.trace "e'",
-  tactic.trace e'.to_raw_fmt,
-  return ()
 
-open tactic expr
 
-example : true := by do
-  t ← mk_meta_var (sort (level.zero.succ)),
-  x ← return $ local_const `x `x binder_info.default t,
-  mt ← infer_type x,
-  trace (to_fmt "mt: " ++ to_fmt mt),
-  e ← to_expr ``(%%x  = 0),
-  get_assignment mt >>= trace
 
+
+
+
+/- create Π and λ from a term and a list of local variables:
+
+expr.pis [l_0 : t_0, …, l_n : t_n] t[l_0, …, l_n] ~>
+  Π(l_0 : t_0) ⋯ (l_n : t_n), t[var n, …, var 0]
+expr.lambda [l_0 : t_0, …, l_n : t_n] t[l_0, …, l_n] ~>
+  λ(l_0 : t_0) ⋯ (l_n : t_n), t[var n, …, var 0]
+
+The `t_i` are allowed to contain `l_j` for `j < i`. The binder also follows the binder info and
+pretty printing name of the local variable.
+-/
+#check expr.pis
+#check expr.lambdas
+
+
+
+
+
+
+
+/- Create a local variable: -/
+#check tactic.mk_local' -- needed to get a unique name
+
+
+
+
+
+
+
+/- Walk into a sequence of Π:
+
+tactic.mk_local_pis (Π(v_0 : t_0)⋯(v_n : t_n),
+  t[var n, …, var 0]) ~>
+  ([v_0, …, v_n], t[v_0, …, v_n])
+-/
+#check tactic.mk_local_pis
+
+
+
+
+
+
+
+end locally_nameless
+
+end vars
+
+end lecture
