meta-prog/tactic_state.lean
@@ -7,127 +7,55 @@ and their corresponding typing context.
 
 open tactic
 
-/- Variables / Constant -/
-section variables
+/- The `tactic` monad allows us to construct expressions, and interact with the user, access
+Lean's environment. The environment contains all declarations (axioms, constant, inductive
+definitions), attribute lists, options, etc... -/
 
-#check (expr.const : name → list level → expr)
-#check (expr.local_const : name → name → binder_info → expr → expr)
-#check (expr.mvar : name → name → expr → expr)
-#check (expr.var : ℕ → expr)
-
-/-
-  * `const`: Constant refering to global declarations, and can be looked up in the name space,
-    they are also universe parametric.
-
-  * `local_const` (Local variables) can be arbitrarily create, but if used to fill in a goal, only
-    local variables from the local context are allowed (including the type!)
-
-  * `mvar` (Meta variables): Holes in our proof / term. Represent the goals we want to solve, or
-    holes to fill in when unifying two terms.
-
-  * `var` (Bound variables): are de-Bruijn indexed, i.e. just a natural number refering to the
-    corresponding lambda.
-
-    Important: When we write a context `C[var 0]`, this doesn't mean that C is a context of `var 0`
-    but `var i` depending on the number of binders it occurs in:
-      In a context `C[*] = λa, * a`:  `C[var 0] ≝ λa, (var 1) a`
-
-Using bound variables with de-Bruijn indices and free variables with names is called a
-**locally nameless representation**.
-
-Local variables and Meta variables exist also in the level representation. They are only used to
-construct a term. In the final declaration local and meta variables do not occur anymore.
-
-Local variables are often used to **walk** into a binder (i.e. a Π or a λ): a new unique name is
-used to create a `local_const` expression using the pretty print name, the binder information, and
-the type of the bound variable. In the expression itself the bound variable is replaced by the local
-variable.
-
-In the interface `expr` is often used to carry all the information of a local constant.
--/
-
-section locally_nameless
-
-/- replace local variables by bound variables
-
-expr.abstract_local C[local_const n _ _ _] n ~> C[var 0]
--/
-#check expr.abstract_local
-#check expr.abstract_locals
-#check expr.abstract
-
-/- instantiate bound variables by terms
-
-expr.instantiate_var C[var 0] t ~> C[t]
--/
-#check expr.instantiate_univ_params
-#check expr.instantiate_var
-#check expr.instantiate_vars
-
-/- instantiate local variables by terms
-
-expr.instantiate_local n t C[local_const n _ _ _] ~> C[t]
--/
-#check expr.instantiate_local
-#check expr.instantiate_locals
-
-/- create Π and λ from a term and a list of local variables:
-
-expr.pis [l_0 : t_0, …, l_n : t_n] t[l_0, …, l_n] ~> Π(l_0 : t_0) ⋯ (l_n : t_n), t[var n, …, var 0]
-expr.lambda [l_0 : t_0, …, l_n : t_n] t[l_0, …, l_n] ~> λ(l_0 : t_0) ⋯ (l_n : t_n), t[var n, …, var 0]
-
-The `t_i` are allowed to contain `l_j` for `j < i`. The binder also follows the binder info and
-pretty printing name of the local variable.
--/
-#check expr.pis
-#check expr.lambdas
+#check tactic
+#print prefix tactic
+#check declaration
+#print prefix declaration
 
 
-/- Create a local variable: -/
-#check tactic.mk_local' -- needed to get a unique name
+-- we can do very basic stuff in the tactic framework
 
-/- Walk into a sequence of Π:
+example {α : Type} : ∀a:α, a = a :=
+begin
+  intro,
+  reflexivity
+end
 
-tactic.mk_local_pis (Π(v_0 : t_0)⋯(v_n : t_n), t[var n, …, var 0]) ~>
-  ([v_0, …, v_n], t[v_0, …, v_n])
--/
-#check tactic.mk_local_pis
-
-end locally_nameless
-
-end variables
-
-section term_construction
-
-/-
-Note on term construction
--------------------------
-
-Many operations are not type checked. It is possible to write tactics which produce type
-incorrect terms and fail at a later stage.
-
--/
-
-example : ℕ := by do
-  -- we contstruct a type incorrect local variable
-  (l : expr) ← return $ expr.local_const `n `n binder_info.default (expr.const `has_add.add []),
-  t ← infer_type l, -- this just returns the type
-  trace t.to_raw_fmt,
-  t ← infer_type (l.app l), -- this produces an error
-  trace t.to_raw_fmt,
-  skip
-
-example : ℕ := by do
-  (l : expr) ← return $ expr.local_const `n `n binder_info.default (expr.const `ℕ []),
-  (m : expr) ← mk_mvar,
-  t ← infer_type (m.app l), -- infer does not unify meta variables
-  trace t.to_raw_fmt,
-  skip
-
-end term_construction
+example {α : Type} : ∀a:α, a = a := by do
+  intro `a,
+  reflexivity
 
 
-/- How does the goal list work?
+
+
+
+
+meta def find (t : expr) : list expr → tactic expr
+| []        := failed
+| (h :: lc) := do
+  t_h ← infer_type h,
+  ((do unify t t_h, return h)
+    <|>
+    find lc)
+
+meta def my_assm : tactic unit := do
+  lc ← local_context,
+  t ← target,
+  h ← find t lc,
+  exact h
+
+example {p q : Prop} (h : p) (h' : q) : q := by do
+  my_assm
+
+
+
+
+
+/- How does the tactic state work?
 
 `set_goals`, `get_goals`: Set and get the list of goals.
   * A goal is not the statement to proof, but the meta variable to fill in.
@@ -184,6 +112,16 @@ Introduce a new name `x.0`:
 
 end intro
 
+
+
+
+
+
+
+
+
+
+
 section apply
 
 /- How `apply r` works:
@@ -198,6 +136,16 @@ Create a meta variable for all additional parameters, i.e. if the goal is
 -/
 
 end apply
+
+
+
+
+
+
+
+
+
+
 
 section induction
 
